proof/invariant-abstract/RISCV64/ArchSyscall_AI.thy
@@ -54,17 +54,19 @@ lemma diminished_no_cap_to_obj_with_diff_ref [Syscall_AI_assms]:
   done
 
 lemma hv_invs[wp, Syscall_AI_assms]: "\<lbrace>invs\<rbrace> handle_vm_fault t' flt \<lbrace>\<lambda>r. invs\<rbrace>"
-  by (cases flt; wpsimp)
+  unfolding handle_vm_fault_def by (cases flt; wpsimp)
 
 crunch inv[wp]: getRegister, read_sbadaddr "P"
   (ignore_del: getRegister)
 
 lemma hv_inv_ex [Syscall_AI_assms]:
   "\<lbrace>P\<rbrace> handle_vm_fault t vp \<lbrace>\<lambda>_ _. True\<rbrace>, \<lbrace>\<lambda>_. P\<rbrace>"
+  unfolding handle_vm_fault_def
   by (cases vp; wpsimp wp: dmo_inv getRestartPC_inv det_getRestartPC as_user_inv)
 
 lemma handle_vm_fault_valid_fault[wp, Syscall_AI_assms]:
   "\<lbrace>\<top>\<rbrace> handle_vm_fault thread ft -,\<lbrace>\<lambda>rv s. valid_fault rv\<rbrace>"
+  unfolding handle_vm_fault_def
   apply (cases ft, simp_all)
    apply (wp | simp add: valid_fault_def)+
   done
@@ -72,11 +74,11 @@ lemma handle_vm_fault_valid_fault[wp, Syscall_AI_assms]:
 
 lemma hvmf_active [Syscall_AI_assms]:
   "\<lbrace>st_tcb_at active t\<rbrace> handle_vm_fault t w \<lbrace>\<lambda>rv. st_tcb_at active t\<rbrace>"
-  by (cases w; wpsimp)
+  unfolding handle_vm_fault_def by (cases w; wpsimp)
 
 lemma hvmf_ex_cap[wp, Syscall_AI_assms]:
   "\<lbrace>ex_nonz_cap_to p\<rbrace> handle_vm_fault t b \<lbrace>\<lambda>rv. ex_nonz_cap_to p\<rbrace>"
-  by (cases b; wpsimp)
+  unfolding handle_vm_fault_def by (cases b; wpsimp)
 
 declare arch_get_sanitise_register_info_ex_nonz_cap_to[Syscall_AI_assms]
 
